src/Lean/Meta/Tactic/Grind/Intro.lean
@@ -55,9 +55,9 @@ It ensures base name is a simple `Name` and does not have a `_<idx>` suffix
 private def mkBaseName (name : Name) (type : Expr) : MetaM Name := do
   if let .str _ s := name then
     let pos := s.find (· == '_')
-    unless pos < s.endPos do
+    unless pos < s.rawEndPos do
       return Name.mkSimple s
-    let suffix := String.Pos.Raw.extract s (pos+'_') s.endPos
+    let suffix := String.Pos.Raw.extract s (pos+'_') s.rawEndPos
     unless suffix.isNat do
       return Name.mkSimple s
     let s := String.Pos.Raw.extract s ⟨0⟩ pos
