src/Lean/PrettyPrinter/Formatter.lean
@@ -389,7 +389,7 @@ def pushToken (info : SourceInfo) (tk : String) (ident : Bool) : FormatterM Unit
         -- Check if we would parse more than `tk` as a single token
         let tk' := tk.trimLeft
         let t ← parseToken $ tk' ++ st.leadWord
-        if t.pos ≤ tk'.endPos then
+        if t.pos ≤ tk'.rawEndPos then
           -- stopped within `tk` => use it as is
           pure false
         else
@@ -612,7 +612,7 @@ def continuation : String := " [...]"
 instance : Std.Format.MonadPrettyFormat M where
   pushOutput s := do
     let lineEnd := s.find (· == '\n')
-    if lineEnd < s.endPos then
+    if lineEnd < s.rawEndPos then
       let s := (String.Pos.Raw.extract s 0 lineEnd).trimRight ++ continuation
       modify fun st => { st with line := st.line.append s }
       throw ()
